vector: extracted results about credits

src/examples/vector.v
@@ -1,16 +1,9 @@
 From stdpp Require Import decidable binders gmultiset.
-From iris.proofmode Require Import proofmode.
-
-From iris.algebra Require Import gmap.
-
-From spacelambda.language Require Import notation.
-
-From spacelambda Require Import more_space_lang wp_all triple.
-
-From spacelambda.examples Require Export tactics utils diaframe.
+From iris Require Import proofmode.proofmode algebra.gmap.
+From spacelambda Require Import language.notation more_space_lang wp_all triple.
+From spacelambda.examples Require Import tactics utils diaframe.
 
 (** TODO move *)
-
 Lemma wp_enc_return_unit_iff `{!interpGS Σ} `{Enc A} b t (Q : iProp Σ) :
   wp_enc b t (λ _ : (), Q) ⊣⊢ wp_enc b t (λ r : val, ⌜r = ()%V⌝ ∗ Q).
 Proof.
@@ -771,70 +764,6 @@ Proof.
   intros ? (?, ?) ?. rewrite -opposite_singleton opposite_cancel //.
 Qed.
 
-(** Cleanup tactic for proving examples *)
-
-Import environments.
-Local Ltac cleanup :=
-  simpl;
-  repeat (
-      match goal with |- envs_entails _ (_ -∗ _) => iIntros "?" end
-     || match goal with |- envs_entails _ (∀ _, _) => iIntros (?) end
-     || match goal with |- envs_entails _ (♢ ?n ∗ _)%I => mine n as "_H"; [ iFrame "_H" | ..] end
-     || iDestruct (diamonds_join with "[$]") as "?"
-     || iDestruct select (_ ∗ _)%I as "(? & ?)"
-     || iDestruct select (⌜_⌝)%I as "%").
-
-Example example `{!interpGS Σ} :
-  CODE (
-      let: "v" := vector_create [[]] in
-      vector_push [["v", ^1]];;
-      vector_push [["v", ^2]];;
-      vector_push [["v", ^3]];;
-      vector_push [["v", ^4]];;
-      vector_push [["v", ^5]];;
-      vector_push [["v", ^6]];;
-      vector_push [["v", ^7]];;
-      vector_set [["v", ^0, ^11]];;
-      vector_set [["v", ^1, ^12]];;
-      vector_set [["v", ^1, ^22]];;
-      vector_pop [["v"]];;
-      vector_pop [["v"]];;
-      vector_pop [["v"]];;
-      vector_pop [["v"]];;
-      vector_pop [["v"]];;
-      let: "x" := vector_pop [["v"]] in
-      "x"
-    )
-  PRE (♢19 ∗ $43)
-  POST (fun res : val => ⌜res = 22⌝ ∗ ♢19 ∗ $0).
-Proof.
-  iIntros "?".
-  cleanup.
-  wps_bind. wps_apply vector_create_spec. cleanup.
-  wps_bind. wps_apply vector_push_spec_no_resize; auto. cleanup.
-  wps_bind. wps_apply vector_push_spec_resize; auto. simpl. cleanup.
-  wps_bind. wps_apply vector_push_spec_resize; auto. simpl. cleanup.
-  wps_bind. wps_apply vector_push_spec_no_resize; auto. cleanup.
-  wps_bind. wps_apply vector_push_spec_resize; auto. simpl. cleanup.
-  wps_bind. wps_apply vector_push_spec_no_resize; auto. cleanup.
-  wps_bind. wps_apply vector_push_spec_no_resize; auto. cleanup.
-  wps_bind. wps_apply vector_set_spec; auto. simpl; lia. cleanup.
-  wps_bind. wps_apply vector_set_spec; auto. simpl; lia. cleanup.
-  wps_bind. wps_apply vector_set_spec; auto. simpl; lia. cleanup.
-  wps_bind. wps_apply vector_pop_joined_specs_lookup; auto. cleanup.
-  wps_bind. wps_apply vector_pop_joined_specs_lookup; auto. cleanup.
-  wps_bind. wps_apply vector_pop_joined_specs_lookup; auto. cleanup.
-  wps_bind. wps_apply vector_pop_joined_specs_lookup; auto. cleanup.
-  wps_bind. wps_apply vector_pop_joined_specs_lookup; auto. cleanup.
-  wps_bind.
-  iApply wps_context_singleton. iFrame.
-  wps_apply vector_pop_joined_specs_lookup; auto. cleanup.
-  iApply (wps_esupd _ _ _ _ (vector_free _ _ _)). iFrame. cleanup.
-  subst. wps_val. iSplit; auto. rew_qz; auto. iFrame.
-Unshelve.
-  all: try exact 1%Qp.
-  set_solver.
-Qed.
 
 (** Amortized specifications *)
 
@@ -852,12 +781,23 @@ Proof.
   iDestruct (time_credit_split with "T") as "($ & $)".
 Qed.
 
+Lemma time_credit_split_3 `{!interpGS Σ} (n m l: nat) :
+  ($ (n + m + l) -∗ $ n ∗ $ m ∗ $ l).
+Proof.
+  iIntros "d".
+  iDestruct (time_credit_split with "[$]") as "(? & $)".
+  iDestruct (time_credit_split with "[$]") as "($ & $)".
+Qed.
+
 Lemma time_credit_weak `{!interpGS Σ} (n m : nat) :
   n <= m -> ($ m -∗ $ n).
 Proof.
   iIntros (L) "T". replace m with (n + (m - n)) by lia.
   iDestruct (time_credit_split with "T") as "($ & _)".
 Qed.
+
+Definition space_reserve (cap size : nat) : nat :=
+  1 + size * 6 - cap.
 
 Definition time_reserve (cap size : nat) : nat :=
   if decide (cap / 2 <= size) then
@@ -868,7 +808,7 @@ Definition time_reserve (cap size : nat) : nat :=
 Definition VectorAm `{!interpGS Σ} (vs : list (val * Qp)) (l : loc) : iProp Σ :=
   ∃ (capacity : nat),
       ⌜ capacity <= 1 `max` (4 * length vs) ⌝
-    ∗ ♢ (1 + length vs * 6 - capacity)%nat
+    ∗ ♢ (space_reserve capacity (length vs))%nat
     ∗ $ (time_reserve capacity (length vs))
     ∗ Vector vs l capacity.
 
@@ -900,6 +840,41 @@ Proof.
   iExists _; iFrame.
 Qed.
 
+Lemma space_reserve_push_no_resize cap size :
+  cap <= 1 `max` (4 * size) ->
+  6 + space_reserve cap size = space_reserve cap (size + 1).
+Proof.
+  unfold space_reserve; lia.
+Qed.
+
+Lemma time_reserve_push_no_resize cap size :
+  time_reserve cap (size + 1) ≤ 6 + time_reserve cap size.
+Proof.
+  unfold time_reserve.
+  do 2 destruct (decide _); lia.
+Qed.
+
+(** TODO consider transforming this into:
+  ♢6 + ♢(reserve...) -∗ ♢(cap * 2) ∗ (♢cap -∗ ♢(reserve ...)) *)
+Lemma space_reserve_push_resize cap :
+  6 + space_reserve cap cap =
+  cap * 2 + (space_reserve (cap * 2) (cap + 1) - cap).
+Proof.
+  unfold space_reserve.
+  lia.
+Qed.
+
+Lemma time_reserve_push_resize size :
+  7 + time_reserve size size =
+    (1 + (size * 3 + 0)) + time_reserve (size * 2) (size + 1) + 3 * (size `mod` 2).
+Proof.
+  unfold time_reserve.
+  rewrite Nat.div_mul //.
+  pose proof Nat.div_mod_eq size 2.
+  pose proof Nat.mod_upper_bound size 2.
+  do 2 destruct (decide _); try lia.
+Qed.
+
 Lemma vector_push_amortized_spec `{!interpGS Σ} vs l v (q : Qp) :
   CODE (vector_push [[#l, v]])
   SOUV {[l]}
@@ -909,41 +884,51 @@ Proof.
   iIntros "(Sv & pv & V & dia & T)".
   iDestruct "V" as (cap) "(%Ucap & dn & dT & V)".
   destruct (decide (length vs < cap)) as [ok|over].
-  - iPoseProof (vector_push_spec_no_resize with "[$]") as "A"; auto.
-    iApply (wps_mono with "A"). iIntros (_) "(V & T)".
-    iExists cap. iFrame.
-    iDestruct (time_credit_join with "[$]") as "T".
-    rewrite app_length //.
+  - (* size < cap: no resize *)
+    wps_apply vector_push_spec_no_resize. auto.
+    iDestruct select (_ ∗ _)%I as "(V & T)".
+    (* re-establish invariant *)
+    iExists cap.
+    iFrame.
     iSplitR.
-    + iPureIntro. lia.
-    + iSplitR "T".
-      * iDestruct (diamonds_join with "[$]") as "?". iApply (diamonds_eq with "[$]"). rew_qz. simpl. lia.
-      * iApply (time_credit_weak with "T"). simpl length.
-        unfold time_reserve. do 2 destruct (decide _); lia.
-  - iAssert ⌜length vs ≤ cap⌝%I as "%". by iDestruct "V" as (?) "(($ & _) & _ & _)".
+    + (* upper bound on cap *)
+      iPureIntro. rewrite app_length. lia.
+    + (* time and space credits *)
+      iDestruct (diamonds_join with "[$]") as "?".
+      rewrite app_length.
+      rew_qz.
+      rewrite space_reserve_push_no_resize // /=.
+      iFrame.
+      iDestruct (time_credit_join with "[$]") as "?".
+      iApply (time_credit_weak with "[$]").
+      apply time_reserve_push_no_resize.
+  - (* size = cap: will resize *)
+    iAssert ⌜length vs ≤ cap⌝%I as "%". by iDestruct "V" as (?) "(($ & _) & _ & _)".
     assert (cap = length vs) as -> by lia.
+    wps_apply vector_push_spec_resize; auto.
+    (* massaging credits to match precondition *)
     iDestruct (diamonds_join with "[$]") as "?".
-    mine (length vs * 2) as "d2".
+    rew_qz.
+    rewrite space_reserve_push_resize nat_to_Qz_add.
+    iDestruct (diamonds_split with "[$]") as "(d2 & ?)".
     iDestruct (time_credit_join with "[$]") as "T".
-    iDestruct (time_credit_split_alt (S (length vs * 3 + 0)) with "[$]") as "(T1 & T)".
-    { unfold time_reserve.
-      pose proof Nat.div_mod_eq (length vs) 2.
-      pose proof Nat.mod_upper_bound (length vs) 2.
-      destruct (decide _); lia. }
-    iPoseProof (vector_push_spec_resize with "[$Sv $pv $V d2 $T1]") as "A"; auto. by rew_qz.
-    iApply (wps_mono with "A"). iIntros (_) "(V & d & T0)".
-    iExists (length vs * 2). iFrame.
+    rewrite time_reserve_push_resize.
+    iDestruct (time_credit_split_3 with "[$]") as "(T1 & T2 & Tjunk)".
+    rew_qz. iFrame.
+    iIntros (_) "(V & d & T0)".
+    (* re-establish invariant *)
+    iExists (length vs * 2).
+    rewrite app_length.
+    iFrame.
     iSplitR.
-    + iPureIntro. rewrite app_length. rew_qz. lia.
-    + iSplitR "T".
-      * iDestruct (diamonds_join with "[$]") as "?".
-        iApply (diamonds_eq with "[$]"). rewrite app_length /= //. rew_qz. lia.
-      * rewrite app_length. simpl length.
-        iApply (time_credit_weak with "T").
-        unfold time_reserve.
-        pose proof Nat.div_mod_eq (length vs) 2.
-        pose proof Nat.div_mul (length vs) 2.
-        do 2 destruct (decide _); lia.
+    + (* upper bound on cap *)
+      iPureIntro. rew_qz. lia.
+    + (* credits *)
+      iDestruct (diamonds_join with "[$]") as "?".
+      iApply (diamonds_eq with "[$]").
+      rew_qz.
+      rewrite /= // /space_reserve.
+      lia.
 Qed.
 
 Lemma vector_set_amortized_spec `{!interpGS Σ} vs l i (x : val) (q : Qp) :
@@ -983,6 +968,51 @@ Proof.
   auto.
 Qed.
 
+Lemma space_reserve_pop_no_resize cap size :
+  cap < 4 * size ->
+  space_reserve cap (size + 1) = 6 + space_reserve cap size.
+Proof.
+  unfold space_reserve.
+  lia.
+Qed.
+
+Lemma space_reserve_pop_resize cap size :
+  cap ≤ 1 `max` (4 * (size + 1)) ->
+  space_reserve cap (size + 1) =
+    (1 `max` (size * 2)) +
+      (((space_reserve (1 `max` (size * 2)) size) + 6) - cap).
+Proof.
+  unfold space_reserve.
+  lia.
+Qed.
+
+Lemma time_reserve_pop_no_resize cap size :
+  cap ≤ 1 `max` (4 * (size + 1)) ->
+  cap < 4 * size ->
+  3 + time_reserve cap (size + 1) =
+  time_reserve cap size + if decide (cap `div` 2 ≤ size) then 9 else 0.
+Proof.
+  unfold time_reserve.
+  pose proof Nat.div_mod_eq size 2.
+  pose proof Nat.mod_upper_bound size 2.
+  do 2 destruct (decide _); lia.
+Qed.
+
+Lemma time_reserve_pop_resize cap size :
+  4 * size ≤ cap ->
+  cap ≤ 1 `max` (4 * (size + 1)) ->
+  4 + time_reserve cap (size + 1) >=
+    (1 + (1 `max` (size * 2)) + (size + 0)) +
+      time_reserve (1 `max` (size * 2)) size.
+Proof.
+  unfold time_reserve.
+  pose proof Nat.div_mod_eq cap 2.
+  pose proof Nat.mod_upper_bound cap 2.
+  pose proof Nat.div_mod_eq (1 `max` (size * 2)) 2.
+  pose proof Nat.mod_upper_bound (1 `max` (size * 2)) 2.
+  do 2 destruct (decide _); lia.
+Qed.
+
 Lemma vector_pop_amortized_spec `{!interpGS Σ} vs l (x : val) (q : Qp) :
   CODE (vector_pop [[#l]])
   SOUV {[l]}
@@ -996,52 +1026,42 @@ Proof.
   iIntros "(V & T)".
   iDestruct "V" as (cap) "(%Ucap & dn & dT & V)".
   destruct (le_lt_dec (4 * length vs) cap) as [L|L].
-  - rewrite app_length in Ucap |- *; rew_qz.
+  - (* cap >= 4*size, so resizing so that pop goes *)
+    rewrite app_length in Ucap |- *; rew_qz.
     simpl length in *.
-    mine (1 `max` (length vs * 2)) as "dia".
+    (* credits necessary for pop *)
+    rewrite space_reserve_pop_resize // nat_to_Qz_add.
+    iDestruct (diamonds_split with "[$]") as "(dia & dn)".
     iDestruct (time_credit_join with "[$]") as "T".
-    iDestruct (time_credit_split_alt (S (1 `max` (length vs * 2)) + (length vs + 0)) with "[$]") as "(T1 & T)".
-    { revert L Ucap. remember (length vs) as s. clear Heqs. intros.
-      unfold time_reserve.
-      pose proof Nat.div_mod_eq cap 2.
-      pose proof Nat.mod_upper_bound cap 2.
-      destruct (decide _); lia. }
-    iPoseProof (vector_pop_spec_resize vs l cap with "[$]") as "A"; auto.
-    iApply (wps_mono with "A").
-    iIntros (?) "($ & $ & $ & V & dc & T0)".
+    (* (throwing away a few time credits sometimes (0, 3, 6, or 8)) *)
+    iDestruct (time_credit_weak with "[$]") as "T".
+    now apply time_reserve_pop_resize; auto.
+    iDestruct (time_credit_split with "[$]") as "(T1 & T)".
+    wps_apply vector_pop_spec_resize; auto.
+    iDestruct select (_ ∗ _)%I as "($ & $ & $ & V & dc & T0)".
     iDestruct (diamonds_join with "[$]") as "?".
     mine 6 as "dia".
     iFrame "dia".
     iExists _; iFrame.
     iSplitR.
     + iPureIntro. lia.
-    + iSplitR "T".
-      * iApply (diamonds_eq with "[$]"). rew_qz. lia.
-      * iApply (time_credit_weak with "T").
-        unfold time_reserve.
-        revert L Ucap. remember (length vs) as s. clear Heqs. intros.
-        pose proof Nat.div_mul s 2.
-        assert (s = 0 \/ s > 0) as [-> | Ps] by lia. by apply le_0_n.
-        replace (1 `max` (s * 2)) with (s * 2) by lia.
-        do 2 destruct (decide _); lia.
+    + iApply (diamonds_eq with "[$]"). unfold space_reserve. rew_qz. lia.
 
-  - rewrite app_length.
-    iPoseProof (vector_pop_spec_no_resize vs l cap with "[$]") as "A"; auto.
-    iApply (wps_mono with "A").
-    iIntros (?) "($ & $ & $ & V & T)".
-    mine 6 as "dia".
-    2: rewrite app_length in Ucap; rew_qz; lia.
-    iFrame "dia".
+  - (* cap < 4*size: no resize necessary *)
+    rewrite app_length.
+    wps_apply vector_pop_spec_no_resize; auto.
+    iDestruct select (_ ∗ _)%I as "($ & $ & $ & V & T)".
+    (* credits *)
+    rewrite space_reserve_pop_no_resize // nat_to_Qz_add.
+    iDestruct (diamonds_split with "[$]") as "($ & dn)".
+    (* re-establish invariant *)
     iExists cap; iFrame.
     iDestruct (time_credit_join with "[$]") as "T".
+    rewrite app_length in Ucap |- *.
     iSplitR.
     + iPureIntro. lia.
-    + iSplitR "T".
-      * iApply (diamonds_eq with "[$]"). rew_qz. lia.
-      * rewrite app_length in Ucap. simpl length in Ucap.
-        iApply (time_credit_weak with "T"). simpl length.
-        unfold time_reserve.
-        do 2 destruct (decide _); lia.
+    + rewrite time_reserve_pop_no_resize //.
+      iDestruct (time_credit_split with "[$]") as "($ & Tjunk)".
 Qed.
 
 Lemma vector_pop_amortized_spec_lookup `{!interpGS Σ} (vs : list (val * Qp)) l :
@@ -1083,68 +1103,5 @@ Proof.
   iModIntro.
   iApply (diamonds_eq with "[$]").
   rew_qz.
-  lia.
-Qed.
-
-Tactic Notation "cleanup" :=
-  simpl;
-  repeat (
-      match goal with |- envs_entails _ (_ -∗ _) => iIntros "?" end
-     || match goal with |- envs_entails _ (∀ _, _) => iIntros (?) end
-     || match goal with |- envs_entails _ (♢ ?n ∗ _)%I => mine n as "_H"; [ iFrame "_H" | ..] end
-     || match goal with |- envs_entails _ ((♢ ?n ∗ _) ∗ _)%I => mine n as "_H"; [ iFrame "_H" | ..] end
-     || match goal with |- envs_entails _ ($ ?n ∗ _)%I => iDestruct (time_credit_split_alt n with "[$]") as "($ & ?)"; [ try lia | ]  end
-     || iDestruct (diamonds_join with "[$]") as "?"
-     || iDestruct select (_ ∗ _)%I as "(? & ?)"
-     || iDestruct select (⌜_⌝)%I as "%").
-
-Example amortized_example `{!interpGS Σ} :
-  CODE (
-      let: "v" := vector_create [[]] in
-      vector_push [["v", ^1]];;
-      vector_push [["v", ^2]];;
-      vector_push [["v", ^3]];;
-      vector_push [["v", ^4]];;
-      vector_push [["v", ^5]];;
-      vector_push [["v", ^6]];;
-      vector_push [["v", ^7]];;
-      vector_set [["v", ^0, ^11]];;
-      vector_set [["v", ^1, ^12]];;
-      vector_set [["v", ^1, ^22]];;
-      vector_pop [["v"]];;
-      vector_pop [["v"]];;
-      vector_pop [["v"]];;
-      vector_pop [["v"]];;
-      vector_pop [["v"]];;
-      let: "x" := vector_pop [["v"]] in
-      "x"
-    )
-  PRE (♢46 ∗ time_credit 73)
-  POST (fun res : val => ⌜res = 22⌝ ∗ ♢46).
-Proof.
-  iIntros "?".
-  wps_bind. wps_apply vector_create_amortized_spec. cleanup.
-  wps_bind. wps_apply vector_push_amortized_spec; auto. cleanup.
-  wps_bind. wps_apply vector_push_amortized_spec; auto. cleanup.
-  wps_bind. wps_apply vector_push_amortized_spec; auto. cleanup.
-  wps_bind. wps_apply vector_push_amortized_spec; auto. cleanup.
-  wps_bind. wps_apply vector_push_amortized_spec; auto. cleanup.
-  wps_bind. wps_apply vector_push_amortized_spec; auto. cleanup.
-  wps_bind. wps_apply vector_push_amortized_spec; auto. cleanup.
-  wps_bind. wps_apply vector_set_amortized_spec. simpl; lia. cleanup.
-  wps_bind. wps_apply vector_set_amortized_spec. simpl; lia. cleanup.
-  wps_bind. wps_apply vector_set_amortized_spec. simpl; lia. cleanup.
-  wps_bind. wps_apply vector_pop_amortized_spec_lookup. auto. cleanup.
-  wps_bind. wps_apply vector_pop_amortized_spec_lookup. auto. cleanup.
-  wps_bind. wps_apply vector_pop_amortized_spec_lookup. auto. cleanup.
-  wps_bind. wps_apply vector_pop_amortized_spec_lookup. auto. cleanup.
-  wps_bind. wps_apply vector_pop_amortized_spec_lookup. auto. cleanup.
-  wps_bind.
-  iApply wps_context_singleton; iFrame.
-  wps_apply vector_pop_amortized_spec_lookup. auto. cleanup.
-  iApply (wps_esupd _ _ _ _ (vector_free_amortized _ v)). iFrame. cleanup.
-  wps_val. iSplit. auto. rew_qz. iFrame.
-Unshelve.
-  all: try exact 1%Qp.
-  subst. auto.
+  unfold space_reserve; lia.
 Qed.
