src/examples/vector_tests.v
@@ -1,0 +1,136 @@
+From stdpp Require Import decidable binders gmultiset.
+From iris Require Import proofmode.proofmode algebra.gmap.
+From spacelambda Require Import language.notation more_space_lang wp_all triple.
+From spacelambda.examples Require Import tactics utils diaframe vector.
+
+(** Examples for non-amortized specifications *)
+
+(** Cleanup tactic for proving examples *)
+
+Import environments.
+Local Ltac cleanup :=
+  simpl;
+  repeat (
+      match goal with |- envs_entails _ (_ -∗ _) => iIntros "?" end
+     || match goal with |- envs_entails _ (∀ _, _) => iIntros (?) end
+     || match goal with |- envs_entails _ (♢ ?n ∗ _)%I => mine n as "_H"; [ iFrame "_H" | ..] end
+     || iDestruct (diamonds_join with "[$]") as "?"
+     || iDestruct select (_ ∗ _)%I as "(? & ?)"
+     || iDestruct select (⌜_⌝)%I as "%").
+
+Example example `{!interpGS Σ} :
+  CODE (
+      let: "v" := vector_create [[]] in
+      vector_push [["v", ^1]];;
+      vector_push [["v", ^2]];;
+      vector_push [["v", ^3]];;
+      vector_push [["v", ^4]];;
+      vector_push [["v", ^5]];;
+      vector_push [["v", ^6]];;
+      vector_push [["v", ^7]];;
+      vector_set [["v", ^0, ^11]];;
+      vector_set [["v", ^1, ^12]];;
+      vector_set [["v", ^1, ^22]];;
+      vector_pop [["v"]];;
+      vector_pop [["v"]];;
+      vector_pop [["v"]];;
+      vector_pop [["v"]];;
+      vector_pop [["v"]];;
+      let: "x" := vector_pop [["v"]] in
+      "x"
+    )
+  PRE (♢19 ∗ $43)
+  POST (fun res : val => ⌜res = 22⌝ ∗ ♢19 ∗ $0).
+Proof.
+  iIntros "?".
+  cleanup.
+  wps_bind. wps_apply vector_create_spec. cleanup.
+  wps_bind. wps_apply vector_push_spec_no_resize; auto. cleanup.
+  wps_bind. wps_apply vector_push_spec_resize; auto. simpl. cleanup.
+  wps_bind. wps_apply vector_push_spec_resize; auto. simpl. cleanup.
+  wps_bind. wps_apply vector_push_spec_no_resize; auto. cleanup.
+  wps_bind. wps_apply vector_push_spec_resize; auto. simpl. cleanup.
+  wps_bind. wps_apply vector_push_spec_no_resize; auto. cleanup.
+  wps_bind. wps_apply vector_push_spec_no_resize; auto. cleanup.
+  wps_bind. wps_apply vector_set_spec; auto. simpl; lia. cleanup.
+  wps_bind. wps_apply vector_set_spec; auto. simpl; lia. cleanup.
+  wps_bind. wps_apply vector_set_spec; auto. simpl; lia. cleanup.
+  wps_bind. wps_apply vector_pop_joined_specs_lookup; auto. cleanup.
+  wps_bind. wps_apply vector_pop_joined_specs_lookup; auto. cleanup.
+  wps_bind. wps_apply vector_pop_joined_specs_lookup; auto. cleanup.
+  wps_bind. wps_apply vector_pop_joined_specs_lookup; auto. cleanup.
+  wps_bind. wps_apply vector_pop_joined_specs_lookup; auto. cleanup.
+  wps_bind.
+  iApply wps_context_singleton. iFrame.
+  wps_apply vector_pop_joined_specs_lookup; auto. cleanup.
+  iApply (wps_esupd _ _ _ _ (vector_free _ _ _)). iFrame. cleanup.
+  subst. wps_val. iSplit; auto. rew_qz; auto. iFrame.
+Unshelve.
+  all: try exact 1%Qp.
+  set_solver.
+Qed.
+
+(** Examples for amortized specifications *)
+
+Tactic Notation "cleanup" :=
+  simpl;
+  repeat (
+      match goal with |- envs_entails _ (_ -∗ _) => iIntros "?" end
+     || match goal with |- envs_entails _ (∀ _, _) => iIntros (?) end
+     || match goal with |- envs_entails _ (♢ ?n ∗ _)%I => mine n as "_H"; [ iFrame "_H" | ..] end
+     || match goal with |- envs_entails _ ((♢ ?n ∗ _) ∗ _)%I => mine n as "_H"; [ iFrame "_H" | ..] end
+     || match goal with |- envs_entails _ ($ ?n ∗ _)%I => iDestruct (time_credit_split_alt n with "[$]") as "($ & ?)"; [ try lia | ]  end
+     || iDestruct (diamonds_join with "[$]") as "?"
+     || iDestruct select (_ ∗ _)%I as "(? & ?)"
+     || iDestruct select (⌜_⌝)%I as "%").
+
+Example amortized_example `{!interpGS Σ} :
+  CODE (
+      let: "v" := vector_create [[]] in
+      vector_push [["v", ^1]];;
+      vector_push [["v", ^2]];;
+      vector_push [["v", ^3]];;
+      vector_push [["v", ^4]];;
+      vector_push [["v", ^5]];;
+      vector_push [["v", ^6]];;
+      vector_push [["v", ^7]];;
+      vector_set [["v", ^0, ^11]];;
+      vector_set [["v", ^1, ^12]];;
+      vector_set [["v", ^1, ^22]];;
+      vector_pop [["v"]];;
+      vector_pop [["v"]];;
+      vector_pop [["v"]];;
+      vector_pop [["v"]];;
+      vector_pop [["v"]];;
+      let: "x" := vector_pop [["v"]] in
+      "x"
+    )
+  PRE (♢46 ∗ time_credit 73)
+  POST (fun res : val => ⌜res = 22⌝ ∗ ♢46).
+Proof.
+  iIntros "?".
+  wps_bind. wps_apply vector_create_amortized_spec. cleanup.
+  wps_bind. wps_apply vector_push_amortized_spec; auto. cleanup.
+  wps_bind. wps_apply vector_push_amortized_spec; auto. cleanup.
+  wps_bind. wps_apply vector_push_amortized_spec; auto. cleanup.
+  wps_bind. wps_apply vector_push_amortized_spec; auto. cleanup.
+  wps_bind. wps_apply vector_push_amortized_spec; auto. cleanup.
+  wps_bind. wps_apply vector_push_amortized_spec; auto. cleanup.
+  wps_bind. wps_apply vector_push_amortized_spec; auto. cleanup.
+  wps_bind. wps_apply vector_set_amortized_spec. simpl; lia. cleanup.
+  wps_bind. wps_apply vector_set_amortized_spec. simpl; lia. cleanup.
+  wps_bind. wps_apply vector_set_amortized_spec. simpl; lia. cleanup.
+  wps_bind. wps_apply vector_pop_amortized_spec_lookup. auto. cleanup.
+  wps_bind. wps_apply vector_pop_amortized_spec_lookup. auto. cleanup.
+  wps_bind. wps_apply vector_pop_amortized_spec_lookup. auto. cleanup.
+  wps_bind. wps_apply vector_pop_amortized_spec_lookup. auto. cleanup.
+  wps_bind. wps_apply vector_pop_amortized_spec_lookup. auto. cleanup.
+  wps_bind.
+  iApply wps_context_singleton; iFrame.
+  wps_apply vector_pop_amortized_spec_lookup. auto. cleanup.
+  iApply (wps_esupd _ _ _ _ (vector_free_amortized _ v)). iFrame. cleanup.
+  wps_val. iSplit. auto. rew_qz. iFrame.
+Unshelve.
+  all: try exact 1%Qp.
+  subst. auto.
+Qed.
